src/Implementations/BatchOperations/Definitions.v
@@ -4,7 +4,7 @@ Fixpoint encrypt_all k vl :=
   match vl with
   | nil => Ret nil
   | v::vl' =>
-    ev <- Encrypt k v;
+    ev <-| Encrypt k v;
     evl' <- encrypt_all k vl';
     Ret (ev::evl')
   end.
@@ -13,7 +13,7 @@ Fixpoint decrypt_all k evl :=
   match evl with
   | nil => Ret nil
   | ev::evl' =>
-    v <- Decrypt k ev;
+    v <-| Decrypt k ev;
     vl' <- decrypt_all k evl';
     Ret (v::vl')
   end.
@@ -22,7 +22,7 @@ Fixpoint write_consecutive a vl :=
   match vl with
   | nil => Ret tt
   | v::vl' =>
-    _ <- Write a v;
+    _ <-| Write a v;
     _ <- write_consecutive (S a) vl';
     Ret tt
   end.
@@ -31,7 +31,7 @@ Fixpoint read_consecutive a count:=
   match count with
   | 0 => Ret nil
   | S count' =>
-    v <- Read a;
+    v <-| Read a;
     vl <- read_consecutive (S a) count';
     Ret (v::vl)
   end.
@@ -39,7 +39,7 @@ Fixpoint read_consecutive a count:=
 Fixpoint write_batch al vl :=
   match al, vl with
   | a::al', v::vl' =>
-    _ <- Write a v;
+    _ <-| Write a v;
     _ <- write_batch al' vl';
     Ret tt            
   | _, _ => Ret tt
@@ -49,7 +49,7 @@ Fixpoint hash_all h vl :=
   match vl with
   | nil => Ret h
   | v::vl' =>
-    h' <- Hash h v;
+    h' <-| Hash h v;
     h'' <- hash_all h' vl';
     Ret h''
   end.
