src/Layers/CacheLayer/Definitions.v
@@ -1,4 +1,4 @@
-Require Import Primitives Simulation Layer.
+Require Import Framework.
 Import ListNotations.
 
 Set Implicit Arguments.
@@ -15,14 +15,14 @@ Set Implicit Arguments.
 
   Definition state := disk value.
   
-  Inductive op : Type -> Type :=
-  | Read : addr -> op (option value)
-  | Write : addr -> value -> op unit
-  | Ret : forall T, T -> op T
-  | Bind : forall T T', op T -> (T -> op T') -> op T'.
+  Inductive prog : Type -> Type :=
+  | Read : addr -> prog (option value)
+  | Write : addr -> value -> prog unit
+  | Ret : forall T, T -> prog T
+  | Bind : forall T T', prog T -> (T -> prog T') -> prog T'.
    
   Inductive exec :
-    forall T, oracle ->  state -> op T -> @Result state T -> Prop :=
+    forall T, oracle ->  state -> prog T -> @Result state T -> Prop :=
   | ExecRead : 
       forall d a,
         exec [Cont] d (Read a) (Finished d (d a))
@@ -32,14 +32,16 @@ Set Implicit Arguments.
         exec [Cont] d (Write a v) (Finished (upd d a v) tt)
 
   | ExecCrash :
-      forall T d (p: op T),
+      forall T d (p: prog T),
         exec [Crash] d p (Crashed d).
 
-  Fixpoint oracle_ok T (p: op T) o (s: state) :=
+  Hint Constructors exec.
+  
+  Fixpoint oracle_ok T (p: prog T) o (s: state) :=
       o = [Cont] \/ o = [Crash].
 
   Theorem exec_deterministic_wrt_oracle :
-    forall o s T (p: op T) ret1 ret2,
+    forall o s T (p: prog T) ret1 ret2,
       exec o s p ret1 ->
       exec o s p ret2 ->
       ret1 = ret2.
@@ -53,7 +55,7 @@ Set Implicit Arguments.
   Qed.
 
   Theorem exec_then_oracle_ok:
-    forall T (p: op T) o s r,
+    forall T (p: prog T) o s r,
       exec o s p r ->
       oracle_ok p o s.
   Proof.
@@ -69,7 +71,7 @@ Module CacheOperation <: Operation.
   Definition oracle := oracle.
   Definition oracle_dec:= list_eq_dec token_dec.
   Definition state := state.
-  Definition op := op.
+  Definition prog := prog.
   Definition exec := exec.
   Definition oracle_ok := oracle_ok.
   Definition exec_deterministic_wrt_oracle :=
@@ -81,7 +83,6 @@ End CacheOperation.
 Module CacheHL := HoareLogic CacheOperation.
 Export CacheHL.
 
-Definition cache_layer_lts := Build_LTS CacheHL.L.oracle state CacheHL.L.prog CacheHL.L.exec.
+Definition cache_layer_lts := Build_LTS CacheHL.Lang.oracle CacheHL.Lang.state CacheHL.Lang.prog CacheHL.Lang.exec.
 
 Notation "p >> s" := (p s) (right associativity, at level 60, only parsing).
-Hint Constructors exec.
