src/Implementations/BatchOperations/Specs.v
@@ -1,0 +1,433 @@
+Require Import Omega.
+Require Import Framework DiskLayer.
+Require Import BatchOperations.Definitions.
+Require Import Datatypes.
+
+Opaque oracle_ok.
+
+Theorem encrypt_all_ok :
+  forall vl k o s F,
+    let kl := fst (fst (fst s)) in
+    let em := snd (fst (fst s)) in
+    let hm := snd (fst s) in
+    << o, s >>
+    PRE: (F * [[ consistent_with_upds em
+             (map (encrypt k) vl) (map (fun v=> (k,v)) vl) ]] >> s)
+    PROG: (encrypt_all k vl)
+    << r, s' >>
+    POST: (F * [[ r = map (encrypt k) vl ]] *
+           [[ fst s' = (kl, upd_batch em r (map (fun v => (k, v)) vl), hm) ]] >> s')%pred
+    CRASH: (F * [[ exists n, fst s' = (kl, upd_batch em (firstn n (map (encrypt k) vl)) (map (fun v => (k, v)) (firstn n vl)), hm) ]] >> s').
+Proof.
+  induction vl; intros; cleanup.
+  {
+    step.
+    simpl; intros; eauto.
+    instantiate (1:=fun s' => F * [[ fst s = fst s']] >> s').
+    simpl; pred_apply; cancel.
+    simpl in *; intros.
+    pred_apply; cancel.
+    exists 0; simpl; eauto.
+    simpl in *; intros; cleanup.
+    pred_apply; cancel.
+  }
+
+  {
+    cleanup. 
+    step.
+    { intros; simpl; pred_apply; cancel. }
+    { intros; simpl in *.
+      instantiate (1:= fun s => F  >> s).
+      simpl; pred_apply; cancel.
+    }
+    { intros; simpl in *.
+      simpl; pred_apply; cancel.
+      exists 0; simpl in *; eauto.
+    } 
+    
+    intros; cleanup.
+    step.
+    { destruct_lifts; intros;
+      pred_apply; cancel; eauto;
+      setoid_rewrite H11; simpl; eauto. }
+    { simpl in *; intros.
+      instantiate (1:= fun s => F >> s).
+      simpl; pred_apply; cancel.
+    }
+    { simpl; intros; pred_apply; cancel.
+      destruct_lifts; cleanup.
+      exists (S x); simpl; setoid_rewrite H14; simpl; eauto.      
+    }
+    
+    intros; simpl in *.
+    destruct_lifts; cleanup.
+    step.
+    {
+      instantiate (1:= fun s => F * [[ fst s = fst s'0]] >> s).
+      intros; simpl; pred_apply; cancel.
+    }
+    {
+      simpl; intros.
+      pred_apply; cancel.
+      exists (S (length vl)); simpl.
+      rewrite firstn_map_comm.
+      rewrite firstn_exact; eauto.
+      cleanup; eauto.
+      setoid_rewrite H15; simpl; eauto.
+    }
+    {
+      simpl in *; intros; cleanup.
+      pred_apply; cancel.
+      cleanup; setoid_rewrite H15; simpl; eauto.
+    }
+    Local Transparent oracle_ok.
+    all: try solve [simpl in *; intros; eauto].
+    instantiate (1:=fun o p s => oracle_ok p o s) in H3; simpl in *; eauto.
+    instantiate (1:= fun _ _ _ _ => True); simpl; eauto.
+    instantiate (1:= fun _ _ _ => True); simpl; eauto.
+    simpl; eauto.
+    Opaque oracle_ok.
+  }
+Qed.
+
+Theorem decrypt_all_ok :
+  forall evl k o s F,
+    let kl := fst (fst (fst s)) in
+    let em := snd (fst (fst s)) in
+    let hm := snd (fst s) in
+    let kvl := get_all_existing em evl in
+    let vl := map snd kvl in
+    << o, s >>
+    PRE: (F * [[ evl = map (encrypt k) vl ]] *
+     [[ repeat k (length evl) = map fst kvl ]] >> s)
+    PROG: (decrypt_all k evl)
+    << r, s' >>
+    POST: (F * [[ r = vl ]] *
+       [[ fst s' = fst s ]] >> s')%pred
+    CRASH: (F * [[ fst s' = fst s ]] >> s').
+Proof.
+  induction evl; intros; cleanup.  
+  { step.
+    instantiate (1:=fun s' => F * [[fst s' = fst s]] >> s').
+    all: simpl; intros; cleanup; try (pred_apply; cancel).
+  }
+  {
+    cleanup. destruct s, p, p.
+    destruct_fresh (m a).
+    {
+      destruct p.
+      simpl fst; simpl snd.
+      step.
+      { simpl in *; intros; cleanup.
+        pred_apply; cancel; cleanup; eauto. }
+      { instantiate (1:= fun s => F >> s); simpl; intros; cleanup.
+        pred_apply; cancel. }
+      { simpl in *; intros; pred_apply; cancel. }
+      
+      intros; cleanup.
+      step.
+      { simpl; intros; destruct_lifts; simpl in *; cleanup.
+        simpl in *.
+        setoid_rewrite H11; clear H11.
+        inversion H12; inversion H13.
+        pred_apply; cancel. }
+      { instantiate (1:= fun s => F >> s); simpl; intros; cleanup.
+        pred_apply; cancel. }
+      { simpl in *; intros; destruct_lifts; cleanup.
+        pred_apply; cancel. }
+
+      simpl in *; intros; destruct_lifts; cleanup.
+      step.
+       {
+         instantiate (1:= fun s => F * [[ fst s = fst s'0]] >> s).
+         intros; simpl; pred_apply; cancel.
+       }
+       {
+         simpl; intros.
+         pred_apply; cancel.
+         cleanup; eauto.
+       }
+       {
+         simpl in *; intros.
+         intuition.
+         pred_apply; cancel.
+         setoid_rewrite H12; simpl; eauto.
+         clear H14 H15; cleanup; eauto.
+       }
+       Local Transparent oracle_ok.
+       all: try solve [simpl in *; intros; eauto].
+       instantiate (1:=fun o p s => oracle_ok p o s) in H3; simpl in *; eauto.
+       instantiate (1:= fun _ _ _ _ => True); simpl; eauto.
+       instantiate (1:= fun _ _ _ => True); simpl; eauto.
+       simpl; eauto.
+       Opaque oracle_ok.
+    }
+    
+    {
+      unfold hoare_triple; intros.
+      destruct_lifts; cleanup.
+      assert (A: length (a :: evl) =
+        length (map (encrypt k)
+                    (map snd (get_all_existing m evl))))
+        by (cleanup; eauto).
+      simpl in A.
+      repeat rewrite map_length in A.
+      pose proof (@get_all_existing_length_le _ _ _ m evl).
+      omega.
+    }
+  }
+Qed.
+
+Theorem hash_all_ok :
+  forall vl h o s F,
+    let kl := fst (fst (fst s)) in
+    let em := snd (fst (fst s)) in
+    let hm := snd (fst s) in
+    let rhl := rolling_hash_list h vl in
+    let hvl := hash_and_pair h vl in
+    << o, s >>
+    PRE: (F * [[ consistent_with_upds hm rhl hvl ]] >> s)
+    PROG: (hash_all h vl)
+    << r, s' >>
+    POST: (F * [[ r = rolling_hash h vl ]] *
+           [[ fst s' = (kl, em, upd_batch hm rhl hvl) ]] >> s')%pred
+    CRASH: (F * [[ exists n, fst s' = (kl, em, upd_batch hm (firstn n rhl) (firstn n hvl)) ]] >> s').
+Proof.
+  induction vl; intros; cleanup.
+  {
+    step.
+    instantiate (1:=fun s' => F * [[fst s' = fst s]] >> s').
+    all: simpl; intros; cleanup; try (pred_apply; cancel).
+    exists 0; simpl; eauto.
+  }
+
+  {
+    cleanup. destruct s, p, p.
+    simpl fst; simpl snd.
+    step.
+    { simpl in *; intros; cleanup.
+      pred_apply; cancel; cleanup; eauto. }
+    { instantiate (1:= fun s => F >> s); simpl; intros; cleanup.
+      pred_apply; cancel. }
+    { simpl in *; intros; pred_apply; cancel.
+      exists 0; simpl; eauto. }
+  
+    intros; cleanup.
+    step.
+    { simpl; intros; destruct_lifts; simpl in *; cleanup.
+      simpl in *.
+      setoid_rewrite H11; clear H11.
+      pred_apply; cancel. }
+    { instantiate (1:= fun s => F >> s); simpl; intros; cleanup.
+      pred_apply; cancel. }
+    { simpl in *; intros; destruct_lifts; cleanup.
+      pred_apply; cancel.
+      exists (S x); setoid_rewrite H11; simpl; eauto. }
+
+     simpl in *; intros; destruct_lifts; cleanup.
+      step.
+       {
+         instantiate (1:= fun s => F * [[ fst s = fst s'0]] >> s).
+         intros; simpl; pred_apply; cancel.
+       }
+       {
+         simpl; intros.
+         pred_apply; cancel.
+         cleanup; eauto.
+         exists (S (length vl)); simpl.
+         rewrite firstn_rolling_hash_list_comm.
+         rewrite firstn_hash_and_pair_comm.
+         rewrite firstn_exact; eauto.         
+         setoid_rewrite H12; simpl; eauto.
+       }
+       {
+         simpl in *; intros.
+         intuition.
+         pred_apply; cancel.
+         cleanup.
+         setoid_rewrite H12; simpl; eauto.
+       }
+       Local Transparent oracle_ok.
+       all: try solve [simpl in *; intros; eauto].
+       instantiate (1:=fun o p s => oracle_ok p o s) in H3; simpl in *; eauto.
+       instantiate (1:= fun _ _ _ _ => True); simpl; eauto.
+       instantiate (1:= fun _ _ _ => True); simpl; eauto.
+       simpl; eauto.
+       Opaque oracle_ok.
+  }
+Qed.
+
+Theorem read_consecutive_ok :
+  forall n start vl o s F,
+    << o, s >>
+      PRE: (F * start |=> vl *
+      [[ length vl = n ]] >> s)
+      PROG: (read_consecutive start n)
+    << r, s' >>
+      POST: (F * start |=> vl *
+       [[ r = map fst vl ]] *
+       [[ fst s' = fst s ]] >> s')%pred
+      CRASH: (F *start |=> vl *
+      [[ fst s' = fst s ]] >> s').
+Proof. Admitted. (*
+  induction n; intros; cleanup.
+  {
+    step.
+    instantiate (1:=fun s' => F * start |=> vl * [[fst s' = fst s]] >> s').
+    all: simpl; intros; cleanup; try (pred_apply; cancel).
+    destruct_lifts; cleanup; simpl; eauto.
+  }
+  
+  {
+    cleanup.
+    destruct vl.
+    {
+      unfold hoare_triple; simpl; intros.
+      repeat destruct_lifts; congruence.
+    }
+    
+    simpl fst; simpl snd.
+    step.
+    { intros; simpl.
+      pred_apply; cancel. }
+    
+    intros; cleanup.
+    step.
+    { apply IHn. }
+    { crush_pimpl. }
+    { crush_pimpl.
+      instantiate (1:= fun _ _ => start |=> (d0::vl)); simpl; cancel. }
+    { crush_pimpl. }
+    
+    step.
+  }
+Qed. *)
+
+Theorem write_consecutive_ok :
+  forall vl start vsl o s F,
+    << o, s >>
+      PRE: (F * start |=> vsl *
+      [[ length vsl = length vl ]] >> s)
+      PROG: (write_consecutive start vl)
+    << r, s' >>
+      POST: (F * start |=> (map_pointwise (map vsupd vl) vsl) *
+       [[ fst s' = fst s ]] >> s')%pred
+      CRASH: ((exists* n, F * start |=> (map_pointwise (map vsupd (firstn n vl)) (firstn n vsl)) *
+             (start + n) |=> skipn n vsl *
+             [[ n <= length vl ]] *
+             [[ fst s' = fst s ]]) >> s').
+Proof. Admitted. (*
+  unfold vsupd; induction vl; intros; cleanup.
+  {
+    step.
+    crush_pimpl.
+    rewrite firstn_nil, skipn_nil; simpl; cancel.
+  }
+  {
+    cleanup.
+    destruct vsl.
+    {
+      unfold hoare_triple; simpl; intros.
+      repeat destruct_lifts; congruence.
+    }
+    
+    simpl fst; simpl snd.
+    step.
+    { intros; simpl.
+      instantiate (1:= fun _ _ => S start |=> vsl * start |-> (a, fst d0 :: snd d0)); simpl; cancel. }
+    { intros; simpl; cancel.
+      eassign 0; simpl; cancel.
+      rewrite Nat.add_0_r; cancel. }
+    
+    step.
+    { apply IHvl. }
+    { crush_pimpl. }
+    { intros; simpl.
+      instantiate (1:= fun _ _ => S start |=> map_pointwise
+        (map (fun v vs => (v, fst vs :: snd vs)) vl) vsl *
+         start |-> (a, fst d0 :: snd d0)); simpl; cancel. }
+    { crush_pimpl.
+      eassign (S n); simpl.
+      rewrite Nat.add_succ_r; cancel.
+      rewrite min_l; eauto; cancel. }
+
+    step.
+    { crush_pimpl.
+      eassign (S (length vsl)); simpl; cancel.
+      rewrite min_l; try omega.
+      repeat rewrite firstn_oob; try omega.
+      rewrite skipn_oob; try omega.
+      simpl; cancel.
+    }
+  }
+  Unshelve.
+  eauto.
+Qed. *)
+
+Theorem write_batch_ok :
+  forall al vl vsl o s F,
+    << o, s >>
+      PRE: (F * al |L> vsl *
+       [[ length vsl = length vl ]] *
+       [[ length al = length vl ]] >> s)
+      PROG: (write_batch al vl)
+    << r, s' >>
+      POST: (F * al |L> (map_pointwise (map vsupd vl) vsl) *
+       [[ fst s' = fst s ]] >> s')%pred
+      CRASH: ((exists* n, F * (firstn n al) |L> (map_pointwise (map vsupd (firstn n vl)) (firstn n vsl)) *
+             (skipn n al) |L> (skipn n vsl) *  
+      [[ fst s' = fst s ]]) >> s').
+Proof. Admitted. (*
+  unfold vsupd; induction al; intros; cleanup.
+  {
+    step.
+    crush_pimpl.
+    eassign 0; simpl; cancel.
+  }
+
+  
+  cleanup.
+  destruct vl.
+  {
+    unfold hoare_triple; simpl; intros.
+    repeat destruct_lifts; congruence.
+  }
+  destruct vsl.
+  {
+    unfold hoare_triple; simpl; intros.
+    repeat destruct_lifts; congruence.
+  }
+  
+  simpl fst; simpl snd.
+  step.
+  { intros; simpl.
+    instantiate (1:= fun _ _ => al |L> vsl * a |-> (v, fst d0 :: snd d0)); simpl; cancel. }
+  { crush_pimpl.
+    eassign 0; simpl; cancel. }    
+  
+  step.
+  { apply IHal. }
+  { crush_pimpl. }
+  { crush_pimpl.
+    instantiate (1:= fun _ _ =>
+       al |L> map_pointwise
+             (map (fun v0 vs => (v0, fst vs :: snd vs)) vl) vsl *
+              a |-> (v, fst d0 :: snd d0)); simpl; cancel. }
+  { crush_pimpl.
+    eassign (S n); simpl; cancel. }
+
+  step.
+  { crush_pimpl.
+    eassign (S (length vl)); simpl; cancel.
+    repeat rewrite firstn_oob; try omega.
+    rewrite skipn_oob; try omega.
+    simpl; cancel.
+  }
+Qed. *)
+
+Hint Extern 1 (hoare_triple _ _ (encrypt_all _ _) _ _ _ _ _ _) => eapply encrypt_all_ok : specs.
+Hint Extern 1 (hoare_triple _ _ (decrypt_all _ _) _ _ _ _ _ _) => eapply decrypt_all_ok : specs.
+Hint Extern 1 (hoare_triple _ _ (hash_all _ _) _ _ _ _ _ _) => eapply hash_all_ok : specs.
+Hint Extern 1 (hoare_triple _ _ (read_consecutive _ _) _ _ _ _ _ _) => eapply read_consecutive_ok : specs.
+Hint Extern 1 (hoare_triple _ _ (write_consecutive _) _ _ _ _ _ _) => eapply write_consecutive_ok : specs.
+Hint Extern 1 (hoare_triple _ _ (write_batch _ _) _ _ _ _ _ _) => eapply write_batch_ok : specs.
