src/Implementations/LogCache/Definitions.v
@@ -1,0 +1,31 @@
+Require Import Datatypes PeanoNat Primitives Log.
+Require Import DiskLayer CacheLayer CachedDiskLayer.
+Import CachedDiskOperation CachedDiskHL.
+
+Axiom addr_list_to_blocks : list addr -> list value.
+
+Definition apply_log := P2 apply_log.
+
+Fixpoint write_batch al vl :=
+  match al, vl with
+  | a::al', v::vl' =>
+    _ <-| P1 (CacheHL.Lang.Op (Write a v));
+    _ <- write_batch al' vl';
+    Ret tt            
+  | _, _ => Ret tt
+  end.
+
+Definition commit addr_l (data_l: list value) :=
+  _ <- write_batch addr_l data_l;
+  _ <-| P2 (commit (addr_list_to_blocks addr_l) data_l);
+  Ret tt.
+
+Definition read a :=
+  mv <-| P1 (CacheHL.Lang.Op (Read a));
+  match mv with
+  | Some v =>
+    Ret v
+  | None =>
+    v <-| P2 (DiskHL.Lang.Op (DiskLayer.Definitions.Read a));
+    Ret v
+  end. 
