src/Layers/CachedDiskLayer/Definitions.v
@@ -1,0 +1,9 @@
+Require Import Framework.
+Require Import DiskLayer CacheLayer.
+Import ListNotations.
+
+Set Implicit Arguments.
+
+Module CachedDiskOperation := HorizontalComposition CacheHL.Lang DiskHL.Lang.
+Module CachedDiskHL := HoareLogic CachedDiskOperation.
+Export CachedDiskHL.
