src/Primitives/Primitives.v
@@ -1,4 +1,0 @@
-Require Export List BaseTypes Mem Pred SepAuto.
-Require Export Disk CommonAutomation ListUtils Primitives.HoareLogic.
-Require Export Primitives.Facts.
-Export ListNotations.
